WIP: multi port max_op

dataplane/Examples/Max_top.thy
@@ -2,248 +2,184 @@ theory Max_top
 
 imports
   "../Timely_Infrastructure"
+  "HOL-Library.Finite_Map"
   Input_top
 begin 
 
 definition "maxs buf = [(n, c) \<leftarrow> buf. n = Max (set (map fst ((filter (\<lambda> (n' :: nat, c'). time c = time c') buf))))]"
 
 (* FIXME: move me *)
-abbreviation "choice4 op1 op2 op3 op4 \<equiv> choice2 (choice2 op1 op2) (choice2 op3 op4)"
+abbreviation "choice5 op1 op2 op3 op4 op5 \<equiv> choice3 (choice2 op1 op2) (choice2 op3 op4) op5"
+
+find_consts "  _ \<Rightarrow>(_ \<times> _) list \<Rightarrow> _ \<Rightarrow> _" 
+
+
+abbreviation "mint_cap os p t \<equiv> os\<lparr> inter := inter os @ [(p, t, 1)] \<rparr>"
 
 
 corec max_top' where
-  "max_top' fron cosm ints prods buf = choice4
-   (Read None (\<lambda> st. if is_Inl st \<and> is_Inr (projl st) then max_top' ((projr (projl st)) (0 :: 1)) cosm ints prods buf else \<oslash>))
-   (let below = [(n, c) \<leftarrow> buf. less_than_frontier fron (time c)] in
-    let result = maxs below in
-    push (max_top' fron cosm ints prods [(n, c) \<leftarrow> buf. \<not> less_than_frontier fron (time c)]) (0 :: 1) result)
-   undefined
-   undefined"
-
-corec max_top' where
-  "max_top' fron cons ints prods buf = choice2
-   (Read (trace (STR ''Reading frontier'') None) (\<lambda> st.
-    if is_Inl st \<and> is_Inr (projl st)
-    then let impf = projr (projl st) in
-      let ft = impf (0 :: 1) in
-      if print_frontier ft  is_empty_antichain ft 
-      then trace (STR ''Empty frontier'') \<oslash> 
-      else let below = [(n, c) \<leftarrow> buf. less_than_frontier ft (time c)] in
-      let result = trace (STR ''Non empty frontier'') (maxs below) in
-      push 
-      (Write (max_top' [(n, c) \<leftarrow> buf. \<not> less_than_frontier ft (time c)]) None (Inl (Inl \<lparr> cons = [], inte = map (\<lambda> c. (out c, time c, -1)) (map snd below), prod = map (\<lambda> c. (out c, time c, 1)) (map snd result) \<rparr>)))
-      (0 :: 1) result
-    else
-      \<oslash>))
-   (pull (1 :: 1) (\<lambda> x. max_top' (buf @ [x])))"
-
+  "max_top' os buf caps = choice5
+   (Read None (\<lambda> st. if is_Inl st \<and> is_Inr (projl st) then max_top' (os\<lparr> front := projr (projl st) \<rparr>) buf caps else \<oslash>))
+   (Choice (cimage (\<lambda> p.
+    let below_caps = [cap \<leftarrow> caps. less_than_frontier (front os p) (time cap)] in
+    let above_caps = [cap \<leftarrow> caps. \<not> less_than_frontier (front os p) (time cap)] in
+    let batches = map (\<lambda> cap. (Max (buf cap), cap)) below_caps in
+    let os' = foldl (\<lambda> os (m, cap). produce os cap [m]) os batches in
+    let os'' = foldl drop_cap os' below_caps in
+    let buf' = foldl (\<lambda> s cap. buf(cap := {})) buf below_caps in
+    Silent (max_top' os'' buf' above_caps)) c\<UU>))
+   (Choice (cimage (\<lambda> p. 
+    Read (Some p)
+    (\<lambda> x. if isl x then \<oslash> else
+     let (n, t) = projr x in
+     let (caps', os') = (if Cap t p \<in> set caps then (caps, os) else (caps @ [Cap t p], mint_cap os p t)) in
+     let buf' = buf((Cap t p) := insert n (buf (Cap t p))) in
+     max_top' os' buf' caps')) c\<UU>))
+    (Choice (cimage (\<lambda> p. (case outpu os p of
+         x # xs \<Rightarrow> send_output (max_top' (os\<lparr> outpu := (outpu os)(p := xs ) \<rparr>) buf caps) p x)) 
+    (cfilter (\<lambda> p. outpu os p \<noteq> []) c\<UU>)))
+    (let (os', st) = obtain_progress os in
+     send_progress (max_top' os' buf caps) st)"
 
 lemma step_max'_top_elim:
-  assumes "step io (max_top' buf) op"
+  assumes "step io (max_top' os buf caps) op"
   obtains
-  x where  "io = Inp None (Inl (Inl x))" "op = \<oslash>"
-| x where  "io = Inp None (Inr x)" "op = \<oslash>"
-| impf ft where "io = Inp None (Inl (Inr impf))" "ft = impf (0 :: 1)"
-  "is_empty_antichain ft" "op = \<oslash>"
-| impf ft below result where "io = Inp None (Inl (Inr impf))" "ft = impf (0 :: 1)"
-  "\<not> is_empty_antichain ft" "below = [(n, c) \<leftarrow> buf. less_than_frontier ft (time c)]" "result = maxs below"
-  "op = push (Write (max_top' [(n, c) \<leftarrow> buf. \<not> less_than_frontier ft (time c)]) None (Inl (Inl \<lparr> cons = [], inte = map (\<lambda> c. (out c, time c, -1)) (map snd below), prod = map (\<lambda> c. (out c, time c, 1)) (map snd result)\<rparr>)) ) 0 result"
-| x t n where "io = Inp (Some 0) (Inr (n, t))"
- "op = Write (max_top' (buf @ [(n, Cap t 1)])) None (Inl (Inl \<lparr> cons = [(1, t, 1)], inte = [(1, t, 1)], prod = [] \<rparr>))"
-| x where "io = Inp (Some 0) (Inl x)" "op = \<oslash>"
+    st where "io = Inp None st" "is_Inl st" "is_Inr (projl st)" "op = max_top' (os\<lparr> front := projr (projl st) \<rparr>) buf caps"
+  | st where "io = Inp None st" "\<not> is_Inl st \<or> \<not> is_Inr (projl st)" "op = \<oslash>"
+  | p above_caps below_caps batches os' os'' buf' where "io = Tau" "below_caps = [cap \<leftarrow> caps. less_than_frontier (front os p) (time cap)]"
+    "above_caps = [cap \<leftarrow> caps. \<not> less_than_frontier (front os p) (time cap)]"
+    "batches = map (\<lambda> cap. (Max (buf cap), cap)) below_caps"
+    "os' = foldl (\<lambda> os (m, cap). produce os cap [m]) os batches"
+    "os'' = foldl drop_cap os' below_caps"
+    "buf' = foldl (\<lambda> s cap. buf(cap := {})) buf below_caps"
+    "op = max_top' os'' buf' above_caps" "p \<notin> defaults"
+  | p x where "io = Inp (Some p) x" "isl x" "op = \<oslash>"
+  | p x n t caps' os' buf' where "io = Inp (Some p) x" "\<not> isl x" "(n, t) = projr x"
+    "(caps', os') = (if Cap t p \<in> set caps then (caps, os) else (caps @ [Cap t p], mint_cap os p t))"
+    "buf' = buf((Cap t p) := insert n (buf (Cap t p)))" "op = max_top' os' buf' caps'"
+  | p x xs where "io = Out (Some p) (Inr x)" "outpu os p = x # xs"
+    "op = max_top' (os\<lparr> outpu := (outpu os)(p := xs ) \<rparr>) buf caps" "p \<notin> defaults"
+  | os' st where "io = Out None (Inl (Inl st))" "obtain_progress os = (os', st)"
+    "op = max_top' os' buf caps"
   using assms apply -
   apply atomize_elim
   apply (subst (asm) max_top'.code)
-  apply (cases io; simp split: option.splits sum.splits if_splits)
+  apply (cases io)
   subgoal for p x
-    apply (cases p; cases x; simp)
-    subgoal for p
-      by (cases p; fastforce)
-    subgoal for p
-      by (cases p; fastforce)
-    subgoal for p
-      by (cases p; fastforce)
-    subgoal for p
-      by (cases p; fastforce)
+    apply simp
+    apply (cases p; simp)
+    subgoal
+      by (auto 0 0 split: if_splits list.splits)
+    subgoal
+      by (fastforce split: prod.splits if_splits list.splits)
     done
-   apply auto
-  done
-
-abbreviation "max_top \<equiv> max_top' []"
-
-abbreviation "ex3 \<equiv> Comp [ (0 :: 2, 0) \<mapsto> (0, 0) ] ex1 (Logic max_top)"
-
-(* value [GHC] "approx_in 32 [VOut (1, 0) (3, 0), VOut (1, 0) (9, 1)] (compile_dataflow ex3)"
- *)
-abbreviation "ex4 \<equiv> Comp (\<lambda> _. None) (Logic (input_top (Cap 0 (1 :: 1)) (LCons [0] LNil))) (Logic (input_top (Cap 0 (1 :: 1)) (LCons [Suc 0] LNil)))"
-
-abbreviation "ex5 \<equiv> Comp (\<lambda> _. None) (Logic (\<I> :: (1 option, 1 option, _) op)) (Logic (\<I> :: (1 option, 1 option, _) op))"
-
-abbreviation "ex6 \<equiv> Comp [ (0 :: 4, 0) \<mapsto> (1, 0), (1, 0) \<mapsto> (0, 0) ] ex4 ex5"
-
-(* value [GHC] "approx_in 15 [VOut (3, 0) (0, 0), VOut (2, 0) (1, 0)] (compile_dataflow ex6)"
- *)
-corec cp_op :: "(1 option, 1 option, 'a) op" where "cp_op = Read (Some 1) (\<lambda>x. Write cp_op (Some 1) x)"
-
-abbreviation "ex7 \<equiv> Comp (\<lambda> _. None) (Logic cp_op) (Logic cp_op)"
-
-abbreviation "ex8 \<equiv> Comp [ (0 :: 4, 0) \<mapsto> (1, 0), (1, 0) \<mapsto> (0, 0) ] ex4 ex7"
-
-(* value [GHC] "approx_in 15 [VOut (3, 0) (0, 0), VOut (2, 0) (1, 0)] (compile_dataflow ex8)"
- *)
-abbreviation "ex9 \<equiv> Comp [ (0, 0) \<mapsto> (1, 0), (1, 0) \<mapsto> (0, 0) ] ex7 ex7"
-
-abbreviation "ex10 \<equiv> Comp [ (0 :: 6, 0) \<mapsto> (1, 0), (1, 0) \<mapsto> (0, 0) ] ex4 ex9"
-
-corec max_op :: "nat \<Rightarrow> _ buf llist \<Rightarrow> (1, 1, _ \<times> nat) op" where
-  "max_op n inps = (case ldropWhile ((=) []) inps of
-     LNil \<Rightarrow> \<oslash>
-   | LCons xs lxs \<Rightarrow> Write (max_op (n + the_enat (llength (ltakeWhile ((=) []) inps))) (LCons xs lxs)) 1 (Max (set xs), n + the_enat (llength (ltakeWhile ((=) []) inps))))"
-
-abbreviation "inp_top c inps \<equiv> map_op (case_option (Inl (0 :: 2)) (\<lambda> p. Inr (0, (p :: 1)))) (case_option (Inl (0 :: 2)) (\<lambda> p. Inr (0, (p :: 1)))) (input_top c inps)"
-abbreviation "m_top buf \<equiv>  map_op (case_option (Inl (1 :: 2)) (\<lambda> p. Inr (1, (p :: 1)))) (case_option (Inl (1 :: 2)) (\<lambda> p. Inr (1, (p :: 1)))) (max_top' buf)"
-
-abbreviation "inp_m_top i inps buf1 buf2 \<equiv> map_op (case_sum id id) (case_sum id id) (comp_op [Inr (0 :: 2, 1 :: 1) \<mapsto> Inr (1, 1)] buf1 (inp_top (Cap i 1) inps) (m_top buf2))"
-
-
-
-
-lemma bisim_step_elim:
-  "op1 ~ op2 \<Longrightarrow>
-   step io op1 op1' \<Longrightarrow>
-   \<exists> op2'. step io op2 op2' \<and> op1' ~ op2'"
-  by (meson bisim.simps sim_def)
-
-fun extract_update where
-  "extract_update (Write op (Inl nid) (Inl (Inl st))) = (Write op (Inl nid) (Inl (Inl \<lparr> cons = [], inte = [], prod = [] \<rparr>)), st)"
-| "extract_update op = (op, \<lparr> cons = [], inte = [], prod = [] \<rparr>)"
-
-abbreviation "no_Choice op \<equiv> is_Read op \<or> is_Write op \<or> is_Silent op"
-
-corec subst_Out_op where
-  "subst_Out_op p x y op = Choice (cimage (\<lambda> op.
-      case op of 
-       Write op' p' x' \<Rightarrow> (if p = p' \<and> x = x' then Write op' p y else Write (subst_Out_op p x y op') p' x')
-     | Read p' f \<Rightarrow> Read p' (\<lambda> x'. (subst_Out_op p x y (f x')))
-     | Silent op' \<Rightarrow> Silent (subst_Out_op p x y op')) (choices op))"
-
-lemma subst_Out_op_cases_simp[simp]:
-  "\<not> is_Read (subst_Out_op p x y op)"
-  "\<not> is_Write (subst_Out_op p x y op)"
-  "\<not> is_Silent (subst_Out_op p x y op)"
-  "is_Choice (subst_Out_op p x y op)"
-  by (subst subst_Out_op.code; simp)+
-
-
-lemma step_subst_op_Tau_intro[intro!]:
-  "step Tau op op' \<Longrightarrow>
-   step Tau (subst_Out_op p x y op) (subst_Out_op p x y op')"
-  apply (erule step_choicesE; simp del: cin.rep_eq)
-    apply (subst subst_Out_op.code)
-  apply force
-  done
-
-lemma step_subst_op_Inp_intro[intro!]:
-  "step (Inp p' x') op op' \<Longrightarrow>
-   step (Inp p' x') (subst_Out_op p x y op) (subst_Out_op p x y op')"
-  apply (erule step_choicesE; simp del: cin.rep_eq)
-    apply (subst subst_Out_op.code)
-  apply force
-  done
-
-lemma step_subst_op_Out_intro1[intro]:
-  "step (Out p x) op op' \<Longrightarrow>
-   step (Out p y) (subst_Out_op p x y op) op'"
-  apply (erule step_choicesE; simp del: cin.rep_eq)
-    apply (subst subst_Out_op.code)
-    apply force
-  done
-
-lemma step_subst_op_Out_intro2[intro]:
-  "step (Out p' x') op op' \<Longrightarrow>
-   x \<noteq> x' \<or> p \<noteq> p' \<Longrightarrow>
-   step (Out p' x') (subst_Out_op p x y op) (subst_Out_op p x y op')"
-  apply (erule step_choicesE; simp del: cin.rep_eq)
-    apply (subst subst_Out_op.code)
-  apply force
-  done
-
-
-lemma step_subst_op_elim[elim]:
-  assumes "step io (subst_Out_op p x y op) op'"
-  obtains 
-    op'' where "step io op op''" "io = Tau" "op' = subst_Out_op p x y op''"
-  | p' x' op'' where "step io op op''" "io = Inp p' x'" "op' = subst_Out_op p x y op''"
-  | p' x' op'' where "step io op op''" "io = Out p' x'" "p \<noteq> p' \<or> x \<noteq> x'" "op' = subst_Out_op p x y op''"
-  | p' x' op'' io' where "step io' op op''" "io' = Out p x" "io = Out p y" "p = p'" "x = x'" "op' = op''"
-  using assms apply atomize_elim
-  apply (subst (asm) subst_Out_op.code)
-  apply (erule step_choicesE)
-  subgoal for p' f x 
-    apply (clarsimp simp del: cin.rep_eq; hypsubst_thin?)
-    subgoal for op'
-      by (cases op'; force split: if_splits)
-    done
-  subgoal for p' x'
-    apply (simp del: de_Morgan_conj cin.rep_eq; hypsubst_thin?)
-    apply (elim cBexE)
-    subgoal for op''
-      by (cases op''; simp del: de_Morgan_conj cin.rep_eq split: if_splits; force)
+  subgoal for p x
+    apply simp
+    apply (cases p; simp)
+    subgoal
+      by (auto 0 0 split: if_splits list.splits)
+    subgoal
+      by (fastforce split: prod.splits if_splits list.splits)
     done
   subgoal
-    apply (clarsimp simp del: cin.rep_eq; hypsubst_thin?)
-    subgoal for op'
-      apply (cases op'; simp del: de_Morgan_conj cin.rep_eq split: if_splits)
-       apply force+
+    by (fastforce split: if_splits list.splits)
+  done
+
+(* 
+  abbreviation "max_top \<equiv> max_top' []"
+*)
+
+term "THE x. P x"
+term "SOME x. P x"
+
+term The
+term Eps
+term the_enat
+
+corec max_op where
+  "max_op n inps = Choice (cimage (\<lambda> p. case ldropWhile ((=) []) (inps p) of
+     LCons xs lxs \<Rightarrow> 
+     Write 
+     (max_op (n(p := n p + the_enat (llength (ltakeWhile ((=) []) (inps p))))) (inps (p := lxs)))
+       p (Max (set xs), n p + the_enat (llength (ltakeWhile ((=) []) (inps p)))))
+     (cfilter (\<lambda> p. ldropWhile ((=) []) (inps p) \<noteq> LNil) c\<UU>))"
+
+
+lemma step_max_op_elim:
+  assumes "step io (max_op n inps) op"
+  obtains p xs lxs where "io = Out p (Max (set xs), n p + the_enat (llength (ltakeWhile ((=) []) (inps p))))" "ldropWhile ((=) []) (inps p) = LCons xs lxs"
+    "op = max_op (n (p := n p + the_enat (llength (ltakeWhile ((=) []) (inps p))))) (inps(p := lxs))" "p \<notin> defaults"
+  using assms apply -
+  apply atomize_elim
+  apply (subst (asm) max_op.code)
+  apply (clarsimp split: llist.splits list.splits)
+  done
+
+lemma step_max_op_Out_intro[intro]:
+  "inps p = LCons xs lxs \<Longrightarrow>
+   xs \<noteq> [] \<Longrightarrow>
+   ys = inps(p := lxs) \<Longrightarrow>
+   p \<notin> defaults \<Longrightarrow>
+   step (Out p (Max (set xs), n p)) (max_op n inps) (max_op n ys)"
+  apply (subst max_op.code)
+  apply (clarsimp split: llist.splits)
+  apply (rule SC)
+   apply (rule cimage_eqI[rotated])
+    apply force
+   apply (rule refl)
+  apply simp
+  apply force
+  done
+
+lemma step_max_op_Out_intro2[intro]:
+  "ldropWhile ((=) []) (inps p) = LCons xs lxs \<Longrightarrow>
+   xs \<noteq> [] \<Longrightarrow>
+   p \<notin> defaults \<Longrightarrow>
+   step (Out p (Max (set xs), (n p) + the_enat (llength (ltakeWhile ((=) []) (inps p))))) (max_op n inps) (max_op (n (p := n p + the_enat (llength (ltakeWhile ((=) []) (inps p))))) (inps(p := lxs)))"
+  apply (subst max_op.code)
+  apply (rule SC)
+   apply (rule cimage_eqI[rotated])
+    apply force
+   apply (rule refl)
+  apply auto
+  done
+
+lemma step_max_op_not_Tau[simp]:
+  "\<not> step Tau (max_op n inps) op"
+  apply (subst max_op.code)
+  apply (auto split: llist.splits list.splits dest!: ldropWhile_LConsD)
+  done
+
+lemma step_max_op_not_Inp[simp]:
+  "\<not> step (Inp p x) (max_op n inps) op"
+  apply (subst max_op.code)
+  apply (auto split: llist.splits list.splits dest!: ldropWhile_LConsD)
+  done
+
+lemma wstep_max_op_simp[simp]:
+  "io \<noteq> Tau \<Longrightarrow>
+   wstep io (max_op n inps) op = step io (max_op n inps) op"
+  unfolding wstep_def
+  apply (cases io; simp)
+  using converse_rtranclpE apply fastforce
+  subgoal
+    apply (rule iffI)
+    subgoal
+      apply clarsimp
+      apply (metis converse_rtranclpE step_max_op_elim step_max_op_not_Tau)
       done
-    done
-  done
-
-coinductive io_ev_inv for io where
-  [intro]: "step io op' op \<Longrightarrow> io_ev_inv io op"
-| [intro]: "(\<And> io' op'. io \<noteq> io' \<Longrightarrow> step io' op op' \<Longrightarrow> io_ev_inv io op') \<Longrightarrow> step io op op' \<Longrightarrow> io_ev_inv io op"
-
-lemma io_ev_map_op:
-  "io_ev_inv io op \<Longrightarrow> map_IO f g id io = io' \<Longrightarrow> io_ev_inv io' (map_op f g op)"
-  apply (coinduction arbitrary: op)
-  subgoal for op
-    apply simp
-    apply (erule io_ev_inv.cases; simp)
-     apply blast
-    apply (rule disjI2)
-    apply (intro conjI[rotated] impI exI allI)
-    apply blast
-    apply (metis step_map_op_elim)
-    done
-  done
-
-lemma io_ev_Out_Inl_comp_op:
-  "io_ev_inv (Out p x) op1 \<Longrightarrow>
-   p \<notin> dom wire \<Longrightarrow>
-   io_ev_inv (Out (Inl p) x) (comp_op wire buf op1 op2)"
-  apply (coinduction arbitrary: buf op1 op2)
-  subgoal for buf op1 op2
-    apply simp
-    apply (erule io_ev_inv.cases; simp)
-    subgoal 
-      by blast
     subgoal
-    apply (rule disjI2)
-    apply (intro conjI[rotated] impI exI allI)
-     apply blast
-    apply (elim step_comp_op_elim; simp; hypsubst_thin; simp)
-           apply force
-          apply force
-         apply force
-        apply force
-    subgoal
-      by blast
-      apply force
-    apply force
-    apply force
+      by auto
     done
   done
-  done
+
+abbreviation "inp_top os caps inps \<equiv> map_op (case_option (Inl (0 :: 2)) (\<lambda> p. Inr (0, p))) (case_option (Inl (0 :: 2)) (\<lambda> p. Inr (0, p))) (input_top os caps inps)"
+abbreviation "m_top os buf caps \<equiv>  map_op (case_option (Inl (1 :: 2)) (\<lambda> p. Inr (1, p))) (case_option (Inl (1 :: 2)) (\<lambda> p. Inr (1, p))) (max_top' os buf caps)"
+
+abbreviation "inp_m_top os1 caps1 inps buf1 os2 buf2 caps2 \<equiv>
+   map_op (case_sum id id) (case_sum id id)
+   (comp_op [(map (\<lambda> p. Inr (0 :: 2, p)) enum_class.enum) [\<mapsto>] (map (\<lambda> p. Inr (1 :: 2, p)) enum_class.enum)] buf1 (inp_top os1 caps1 inps) (m_top os2 buf2 caps2))"
+
 
 (* FIXME: move me *)
 lemma dataflow_op_extract_progress_append:
@@ -260,7 +196,6 @@ lemma propagate_pointstamps_comm:
   "propagate_pointstamps summary conf (cbs1 @ cbs2) = propagate_pointstamps summary conf (cbs2 @ cbs1)"
     unfolding propagate_pointstamps_def Let_def
     by (simp add: change_multiplicities_comm)
-
 
 lemma propagate_pointstamps_append:
   "propagate_pointstamps summary conf cbs1 = Some conf' \<Longrightarrow>
@@ -282,174 +217,20 @@ lemma propagate_pointstamps_append:
     sorry
   done
 
-lemma
-  "(frontier \<circ>\<circ> c_imp) (the (propagate_pointstamps summary conf A)) =
-   (frontier \<circ>\<circ> c_imp) (the (propagate_pointstamps summary conf B)) \<Longrightarrow>
-   (frontier \<circ>\<circ> c_imp) (the (propagate_pointstamps summary conf (A @ C))) =
-   (frontier \<circ>\<circ> c_imp) (the (propagate_pointstamps summary conf (B @ C)))"
-  apply (induct C arbitrary: A B conf)
-  subgoal
-    by simp
-  subgoal for x xs A B conf
-    apply (drule meta_spec[of _ "A @ [x]"])
-    apply (drule meta_spec[of _ "B @ [x]"])
-    apply (drule meta_spec[of _ conf])
-    apply (drule meta_mp)
-    apply (subst (1 2) propagate_pointstamps_append)
-       defer
-       defer
-    apply (rule refl)
-      apply simp
-    oops
-
-lemma aux:
-  "(frontier \<circ>\<circ> c_imp) (the (propagate_pointstamps (summ sg) (pt_tr sg) (lo_pt sg))) =
-   (frontier \<circ>\<circ> c_imp) (the (propagate_pointstamps (summ sg) (pt_tr sg) (lo_pt sg @ extract_progress nid (edges sg) \<lparr>cons = cs, inte = is, prod = ps\<rparr>))) \<Longrightarrow>
-    dataflow_op sg op ~
-    dataflow_op (sg\<lparr>lo_pt := lo_pt sg @ extract_progress nid (edges sg) \<lparr>cons = cs, inte = is, prod = ps\<rparr>\<rparr>)
-     (subst_Out_op (Inl nid) (Inl (Inl \<lparr>cons = cs @ cs', inte = is @ is', prod = ps @ ps'\<rparr>)) (Inl (Inl \<lparr>cons = cs', inte = is', prod = ps'\<rparr>)) op)"
-proof (coinduction arbitrary: sg op rule: bisim_coinduct)
-  case SIM1
-  then show ?case 
-    apply -                
-    apply (elim step_dataflow_op_elim; simp)
-    subgoal for nida p op'' x
-      apply (intro exI conjI[rotated])
-       apply (rule b_base)
-       apply (intro exI conjI)
-         apply (rule refl)+
-       apply hypsubst_thin
-      subgoal 
-         apply force+
-        done
-      subgoal
-        by blast
-      done
-    subgoal
-      apply (intro exI conjI[rotated])
-       apply (rule b_base)
-       apply (intro exI conjI)
-         apply (rule refl)+
-       apply hypsubst_thin
-      subgoal 
-         apply force+
-        done
-      subgoal
-        by blast
-      done
-    subgoal
-      apply (intro exI conjI[rotated])
-       apply (rule b_base)
-       apply (intro exI conjI)
-         apply (rule refl)+
-       apply hypsubst_thin
-      subgoal 
-         apply force+
-        done
-      subgoal
-        by blast
-      done
-    subgoal for nid' op'' st'
-      apply hypsubst_thin
-      apply (cases "nid' = nid \<and> st' = \<lparr>cons = cs @ cs', inte = is @ is', prod = ps @ ps'\<rparr>")
-      subgoal
-        apply (elim conjE; hypsubst_thin)
-        apply (intro exI conjI)
-         apply (rule step_Tau_dataflow_op_Out_Inl_intro[where nid=nid])
-          apply (rule step_subst_op_Out_intro1)
-          apply assumption
-         apply (rule refl)
-        apply simp
-        apply (subgoal_tac 
-    "(dataflow_op (sg\<lparr>lo_pt := lo_pt sg @ extract_progress nid (edges sg) \<lparr>cons = cs, inte = is, prod = ps\<rparr> @ extract_progress nid (edges sg) \<lparr>cons = cs', inte = is', prod = ps'\<rparr>\<rparr>) op'') =
-     (dataflow_op (sg\<lparr>lo_pt := lo_pt sg @ extract_progress nid (edges sg) \<lparr>cons = cs @ cs', inte = is @ is', prod = ps @ ps'\<rparr>\<rparr>) op'')")
-         apply force
-        apply (rule dataflow_op_change_multiplicities)
-           apply simp_all
-        unfolding extract_progress_def
-        apply simp
-        apply (smt (verit, del_insts) change_multiplicities_append change_multiplicities_comm)
-        done
-      subgoal
-        apply (intro exI conjI)
-        apply blast
-        apply (rule b_base)
-        apply (intro conjI exI)
-          apply (rule refl)+
-        defer
-        subgoal 
-          apply simp
-          oops
-(* 
-end
-              apply (subst propagate_pointstamps_append[symmetric])
-              defer
-
-            term minimal_antichain
-
-              find_theorems frontier c_imp
-              
-              sorry
-            done
-          done
-        apply simp
-        apply (rule dataflow_op_change_multiplicities)
-           apply simp_all
-        apply (metis (no_types, lifting) change_multiplicities_append change_multiplicities_comm)
-        done
-      done
-    subgoal for nid' op'' imp_fron sg'
-      apply (simp_all split: option.splits)
-      apply hypsubst_thin
-      apply (intro exI conjI)
-        apply (rule step_Tau_dataflow_op_Inp_Inl_intro)
-          apply (rule step_subst_op_Inp_intro)
-      apply assumption
-         apply (rule refl)+
-      subgoal for conf
-        apply simp
-        sorry
-      subgoal for conf
-        apply simp
-        apply (rule b_base)
-        apply (intro conjI exI)
-         apply (rule refl)+
-          apply simp_all
-        apply (rule dataflow_op_propagate_pointstamps)
-            apply simp_all
-        using propagate_pointstamps_append apply force
-        done
-      done
-    subgoal
-      by blast
-    subgoal
-      by blast
-    subgoal
-      by blast
-    done
-next
-  case SIM2
-  then show ?case sorry
-qed
- *)
-
-lemma aux:
-  "op ~ subst_Out_op (Inl nid) (Inl (Inl \<lparr>cons = cs @ cs', inte = is @ is', prod = ps @ ps'\<rparr>)) (Inl (Inl \<lparr>cons = cs', inte = is', prod = ps'\<rparr>)) op' \<Longrightarrow>
-   dataflow_op sg op ~
-   dataflow_op (sg\<lparr>lo_pt := lo_pt sg @ extract_progress nid (edges sg) \<lparr>cons = cs, inte = is, prod = ps\<rparr>\<rparr>)
-     (subst_Out_op (Inl nid) (Inl (Inl \<lparr>cons = cs @ cs', inte = is @ is', prod = ps @ ps'\<rparr>)) (Inl (Inl \<lparr>cons = cs', inte = is', prod = ps'\<rparr>)) op')"
-  sorry
+(* edges sg = (\<lambda> l. if node l = 0 \<and> port l = Src 1 then [Loc 1 (Trg 0)] else []) \<Longrightarrow> *)
 
 lemma
-  \<open>ys @@- xs @@- lconcat (lmap (\<lambda> (xs, t). map (\<lambda> n. (n, t)) xs) (lzip inps1 (iterates Suc i))) =
-   lconcat (lmap (\<lambda> (xs, t). map (\<lambda> n. (n, t)) xs) (lzip inps2 (iterates Suc j))) \<Longrightarrow>
-   inrbufs1 = buf1 (Inr (1, 1)) \<Longrightarrow>
-   \<forall> x \<in> set inrbufs1. is_Inr x \<Longrightarrow>
-   xs = map projr inrbufs1 \<Longrightarrow>
-   ys = map (\<lambda> (n, c). (n, time c)) buf2 \<Longrightarrow>
-   edges sg = (\<lambda> l. if node l = 0 \<and> port l = Src 1 then [Loc 1 (Trg 0)] else []) \<Longrightarrow>
-   dataflow_op sg (inp_m_top i inps1 buf1 buf2) \<approx>
-   map_op (\<lambda> p. (1, p)) (\<lambda> p. (1, p)) (max_op j inps2)\<close>
+  \<open>input_invar (\<lambda> p. n p + length (xs1 p) + length (xs2 p)) xs3 (outpu os1) \<Longrightarrow>
+   input_invar (\<lambda> p. n p + length (xs1 p)) xs2 (map projr o buf1 o Inr o Pair 1) \<Longrightarrow>
+   dataflow_op sg (inp_m_top os1 (\<lambda> p. n p + length (xs1 p) + length (xs2 p) + length (xs3 p)) inps buf1 os2 buf2 caps2) \<approx>
+   map_op (\<lambda> p. (1, p)) (\<lambda> p. (1, p)) (max_op n (\<lambda> p. xs1 p @@- xs2 p @@- xs3 p @@- inps p))\<close>
+  term "outpu os1"
+  term buf2
+  term xs3
+  term "outpu os1"
+
+  term "\<lambda> c. case c of Cap t p \<Rightarrow> (buf2 )"
+
 proof (coinduction arbitrary: inps1 inps2 buf1 buf2 inrbufs1 xs ys i j sg rule: weakBisimWeakUptoBisim)
   case SIM2
   then show ?case
